WarblreEquiv/LWParameters.v
@@ -73,11 +73,11 @@ Section LWParameters.
   
 
   (* Some lemmas *)
-  Lemma contains_all:
+  (* Lemma contains_all:
     forall c, CharSet.contains Characters.all c = true.
   Proof.
     intro c. rewrite CharSet.contains_spec. unfold Characters.all. rewrite CharSet.from_list_spec. apply char_all_in.
-  Qed.
+  Qed. *)
 
   Lemma from_list_contains_inb: forall (c: Character) (l: list Character), CharSet.contains (CharSet.from_list l) c = List.inb c l.
   Proof.
